specs/Spec.Hash.Helpers.fst
@@ -129,6 +129,14 @@ let pad0_length (a:hash_alg) (len:nat): Tot (n:nat{(len + 1 + n + size_len_8 a) 
 let pad_length (a: hash_alg) (len: nat): Tot (n:nat { (len + n) % size_block a = 0 }) =
   pad0_length a len + 1 + size_len_8 a
 
+#push-options "--max_fuel 0 --max_ifuel 0 --z3rlimit 100"
+let pad_invariant_block (a: hash_alg) (blocks: nat) (rest: nat): Lemma
+  (requires blocks % size_block a = 0)
+  (ensures (pad_length a rest = pad_length a (blocks + rest)))
+  [ SMTPat (pad_length a (blocks + rest)) ]
+=
+  ()
+#pop-options
 
 (** Endian-ness *)
 
