providers/evercrypt/EverCrypt.HMAC.fsti
@@ -46,7 +46,7 @@ val compute:
     live h1 key /\
     live h1 data /\
     LowStar.Modifies.(modifies (loc_buffer tag) h0 h1) /\
-    length data + size_block a <= max_input8 a /\ (* required for subtyping the RHS below *)
+    length data + size_block a < max_input8 a /\ (* required for subtyping the RHS below *)
     as_seq h1 tag == hmac a (as_seq h0 key) (as_seq h0 data))
 
 //18-07-13 pick uniform names? hash{spec} vs compute{hmac}
